Counter.v
@@ -11,36 +11,44 @@ Import ListNotations.
 Section Counter.
 
   Inductive Counter_query :=
-  | CntInc (pid : nat)
-  | CntRead (pid : nat)
+  | CntInc
+  | CntRead
   .
 
   Inductive Counter_reply :=
-  | CntIncOk (pid : nat)
-  | CntReadOk (pid : nat) (value : nat)
+  | CntIncOk
+  | CntReadOk (value : nat)
   .
+
+  Definition li_counter_valid_query_reply : Counter_query -> Counter_reply -> Prop :=
+    fun q r => match q, r with
+    | CntInc, CntIncOk => True
+    | CntRead, CntReadOk _ => True
+    | _, _ => False
+    end.
 
   Definition li_counter :=
     {|
       query := Counter_query;
       reply := Counter_reply;
+      valid_query_reply := li_counter_valid_query_reply;
     |}.
 
   Inductive Internal := 
   | int_cnt_inc
   | int_cnt_read.
 
-  Inductive Invocation :=
+  (* Inductive Invocation :=
   | Inv_Inc
   | Inv_Read.
 
   Inductive Response :=
   | Res_Inc
-  | Res_Read (value : nat).
+  | Res_Read (value : nat). *)
 
   Record Counter_state := mkCntState {
-    requests : LibEnv.env Invocation; 
-    responses : LibEnv.env Response;
+    requests : LibEnv.env Counter_query; 
+    responses : LibEnv.env Counter_reply;
     value : nat
   }.
 
@@ -50,48 +58,48 @@ Section Counter.
 
   Import LibEnv.
 
-  Inductive counter_initial_state : Counter_state -> query li_counter -> Counter_state -> Prop :=
+  Inductive counter_initial_state : Counter_state -> Pid -> query li_counter -> Counter_state -> Prop :=
   | counter_initial_state_inc : forall pid st st' inv res v,
     pid # inv -> pid # res ->
     st = mkCntState inv res v ->
-    st' = mkCntState ((pid, Inv_Inc)::inv) res v ->
-    counter_initial_state st (CntInc pid) st'
+    st' = mkCntState ((pid, CntInc)::inv) res v ->
+    counter_initial_state st pid CntInc st'
   | counter_initial_state_read : forall pid st st' inv res v,
     pid # inv -> pid # res ->
     st = mkCntState inv res v ->
-    st' = mkCntState ((pid, Inv_Read)::inv) res v ->
-    counter_initial_state st (CntRead pid) st'
+    st' = mkCntState ((pid, CntRead)::inv) res v ->
+    counter_initial_state st pid CntRead st'
   .
 
-  Inductive counter_final_state : Counter_state -> reply li_counter -> Counter_state -> Prop :=
+  Inductive counter_final_state : Counter_state -> Pid -> reply li_counter -> Counter_state -> Prop :=
   | counter_final_state_inc : forall pid inv res res' res'' v st st',
-    res = res' ++ [(pid, Res_Inc)] ++ res'' ->
+    res = res' ++ [(pid, CntIncOk)] ++ res'' ->
     st = mkCntState inv res v ->
     st' = mkCntState inv (res' ++ res'') v ->
-    counter_final_state st (CntIncOk pid) st'
+    counter_final_state st pid CntIncOk st'
   | counter_final_state_read : forall pid inv res res' res'' v st st' ret,
-    res = res' ++ [(pid, Res_Read ret)] ++ res'' ->
+    res = res' ++ [(pid, CntReadOk ret)] ++ res'' ->
     st = mkCntState inv res v ->
     st' = mkCntState inv (res' ++ res'') v ->
-    counter_final_state st (CntReadOk pid ret) st'
+    counter_final_state st pid (CntReadOk ret) st'
   .
 
-  Inductive counter_step : Counter_state -> Internal -> Counter_state -> Prop :=
+  Inductive counter_step : Counter_state -> Pid -> Internal -> Counter_state -> Prop :=
   | counter_step_inc : forall pid st st' inv inv' inv'' res v,
-    inv = inv' ++ [(pid, Inv_Inc)] ++ inv'' ->
+    inv = inv' ++ [(pid, CntInc)] ++ inv'' ->
     st = mkCntState inv res v ->
-    st' = mkCntState (inv' ++ inv'') ((pid, Res_Inc)::res) (S v) ->
-    counter_step st int_cnt_inc st'
+    st' = mkCntState (inv' ++ inv'') ((pid, CntIncOk)::res) (S v) ->
+    counter_step st pid int_cnt_inc st'
   | counter_step_read : forall pid st st' inv inv' inv'' res v,
-    inv = inv' ++ [(pid, Inv_Read)] ++ inv'' ->
+    inv = inv' ++ [(pid, CntRead)] ++ inv'' ->
     st = mkCntState inv res v ->
-    st' = mkCntState (inv' ++ inv'') ((pid, Res_Read v)::res) v ->
-    counter_step st int_cnt_read st' 
+    st' = mkCntState (inv' ++ inv'') ((pid, CntReadOk v)::res) v ->
+    counter_step st pid int_cnt_read st' 
   .
 
-  Inductive counter_at_external : Counter_state -> query li_null -> Counter_state -> Prop :=.
+  Inductive counter_at_external : Counter_state -> Pid -> query li_null -> Counter_state -> Prop :=.
 
-  Inductive counter_after_external : Counter_state -> reply li_null -> Counter_state -> Prop :=.
+  Inductive counter_after_external : Counter_state -> Pid -> reply li_null -> Counter_state -> Prop :=.
 
   Definition counter : lts li_null li_counter := mkLTS li_null li_counter
     Counter_state
