Refinement.v
@@ -24,8 +24,8 @@ Inductive valid_execution_fragment (st st' : L.(state)) : list event -> Prop :=
 | Step_None :
     st = st' ->
     valid_execution_fragment st st' nil
-| Step_Internal : forall st'' acts (int : L.(internal)),
-    step L st int st'' ->
+| Step_Internal : forall st'' acts (int : L.(internal)) pid,
+    step L st pid int st'' ->
     valid_execution_fragment st'' st' acts ->
     valid_execution_fragment st st' acts
 (* | Step_At_External : forall st'' acts qa,
@@ -37,12 +37,12 @@ Inductive valid_execution_fragment (st st' : L.(state)) : list event -> Prop :=
     after_external L st ra st'' ->
     valid_execution_fragment st'' st' acts ->
     valid_execution_fragment st st' (event_resA ra :: acts) *)
-| Step_Initial_Call : forall st'' acts qb,
-    initial_state L st qb st'' ->
+| Step_Initial_Call : forall st'' acts qb pid,
+    initial_state L st pid qb st'' ->
     valid_execution_fragment st'' st' acts ->
     valid_execution_fragment st st' (event_inv qb :: acts)
-| Step_Final_Return : forall st'' acts rb,
-    final_state L st rb st'' ->
+| Step_Final_Return : forall st'' acts rb pid,
+    final_state L st pid rb st'' ->
     valid_execution_fragment st'' st' acts ->
     valid_execution_fragment st st' (event_res rb :: acts)
 .
@@ -89,25 +89,25 @@ Definition invariant (P : state L -> Prop) :=
 *)
 Definition invariant_ind (P : state L -> Prop) :=
   (forall st, L.(new_state) st -> P st) /\
-  (forall st st' act,
+  (forall st st' act pid,
     P st ->
-    step L st act st' ->
+    step L st pid act st' ->
     P st') /\
-  (forall st st' act,
+  (forall st st' act pid,
     P st ->
-    initial_state L st act st' ->
+    initial_state L st pid act st' ->
     P st') /\
-  (forall st st' act,
+  (forall st st' act pid,
     P st ->
-    at_external L st act st' ->
+    at_external L st pid act st' ->
     P st') /\
-  (forall st st' act,
+  (forall st st' act pid,
     P st ->
-    after_external L st act st' ->
+    after_external L st pid act st' ->
     P st') /\
-  (forall st st' act,
+  (forall st st' act pid,
     P st ->
-    final_state L st act st' ->
+    final_state L st pid act st' ->
     P st').
 
 End Trace.
@@ -136,13 +136,13 @@ Record fsim_properties (L1 L2 : lts li_null liB)
       forall s1, new_state L1 s1 -> 
       exists s2, new_state L2 s2 /\ match_states s1 s2;
     fsim_match_initial_states:
-      forall s1 s1' s2 qb, match_states s1 s2 -> initial_state L1 s1 qb s1' ->
-      exists s2', initial_state L2 s2 qb s2' /\ match_states s1' s2';
+      forall s1 s1' s2 qb pid, match_states s1 s2 -> initial_state L1 s1 pid qb s1' ->
+      exists s2' pid', initial_state L2 s2 pid' qb s2' /\ match_states s1' s2';
     fsim_match_final_states:
-      forall s1 s1' s2 rb, match_states s1 s2 -> final_state L1 s1 rb s1' ->
-      exists s2', final_state L2 s2 rb s2' /\ match_states s1' s2';
+      forall s1 s1' s2 rb pid, match_states s1 s2 -> final_state L1 s1 pid rb s1' ->
+      exists s2' pid', final_state L2 s2 pid' rb s2' /\ match_states s1' s2';
     fsim_simulation:
-      forall s1 s1' s2 int, match_states s1 s2 -> step L1 s1 int s1' ->
+      forall s1 s1' s2 int pid, match_states s1 s2 -> step L1 s1 pid int s1' ->
       exists s2', valid_execution_fragment L2 s2 s2' [] /\ match_states s1' s2'
   }.
 
@@ -152,11 +152,11 @@ Definition fsim_properties_inv_ind (L1 L2 : lts li_null liB)
   (invariant_ind _ inv) /\
       (forall s1, new_state L1 s1 -> 
       exists s2, new_state L2 s2 /\ match_states s1 s2) /\
-      (forall s1 s1' s2 qb, inv s1 -> match_states s1 s2 -> initial_state L1 s1 qb s1' ->
-      exists s2', initial_state L2 s2 qb s2' /\ match_states s1' s2') /\
-      (forall s1 s1' s2 rb, inv s1 -> match_states s1 s2 -> final_state L1 s1 rb s1' ->
-      exists s2', final_state L2 s2 rb s2' /\ match_states s1' s2') /\
-      (forall s1 s1' s2 int, inv s1 -> match_states s1 s2 -> step L1 s1 int s1' ->
+      (forall s1 s1' s2 qb pid, inv s1 -> match_states s1 s2 -> initial_state L1 s1 pid qb s1' ->
+      exists s2' pid', initial_state L2 s2 pid' qb s2' /\ match_states s1' s2') /\
+      (forall s1 s1' s2 rb pid, inv s1 -> match_states s1 s2 -> final_state L1 s1 pid rb s1' ->
+      exists s2' pid', final_state L2 s2 pid' rb s2' /\ match_states s1' s2') /\
+      (forall s1 s1' s2 int pid, inv s1 -> match_states s1 s2 -> step L1 s1 pid int s1' ->
       exists s2', valid_execution_fragment L2 s2 s2' [] /\ match_states s1' s2')
   .
 
@@ -180,7 +180,7 @@ Proof.
     assert (inv st) as Hinvst by eauto.
     assert (inv st'') as Hinvst'' by eauto.
     destruct Hrel_trace as [Hrel_trace_init [Hrel_trace_final Hrel_trace_step]].
-    specialize (Hrel_trace_step st st'' s2' int Hinvst Hrel H).
+    specialize (Hrel_trace_step st st'' s2' int pid Hinvst Hrel H).
     inversion Hrel_trace_step as [s2'' [Hs2''rel Hs2''valid]].
     specialize (IHHtrace1 Hinvst'' s2'' Hs2''valid).
     inversion IHHtrace1 as [s2 Hs2].
@@ -190,8 +190,8 @@ Proof.
     assert (inv st) as Hinvst by eauto.
     assert (inv st'') as Hinvst'' by eauto.
     destruct Hrel_trace as [Hrel_trace_init [Hrel_trace_final Hrel_trace_step]].
-    specialize (Hrel_trace_init st st'' s2' qb Hinvst Hrel H).
-    inversion Hrel_trace_init as [s2'' [Hs2''rel Hs2''valid]].
+    specialize (Hrel_trace_init st st'' s2' qb pid Hinvst Hrel H).
+    inversion Hrel_trace_init as [s2'' [pid' [Hs2''rel Hs2''valid]]].
     specialize (IHHtrace1 Hinvst'' s2'' Hs2''valid).
     inversion IHHtrace1 as [s2 Hs2].
     eexists; subst; intuition; eauto.
@@ -200,8 +200,8 @@ Proof.
     assert (inv st) as Hinvst by eauto.
     assert (inv st'') as Hinvst'' by eauto.
     destruct Hrel_trace as [Hrel_trace_init [Hrel_trace_final Hrel_trace_step]].
-    specialize (Hrel_trace_final st st'' s2' rb Hinvst Hrel H).
-    inversion Hrel_trace_final as [s2'' [Hs2''rel Hs2''valid]].
+    specialize (Hrel_trace_final st st'' s2' rb pid Hinvst Hrel H).
+    inversion Hrel_trace_final as [s2'' [pid' [Hs2''rel Hs2''valid]]].
     specialize (IHHtrace1 Hinvst'' s2'' Hs2''valid).
     inversion IHHtrace1 as [s2 Hs2].
     eexists; subst; intuition; eauto.
