Register.v
@@ -2,7 +2,7 @@ Require Import
   List
   Nat
   LTS.
-Require LibEnv.
+From VCO Require LibEnv.
 Import ListNotations.
 
 (* 
@@ -25,32 +25,40 @@ Section Register.
     who calls to or returns from Register.
   *)
   Inductive Register_query :=
-  | RegCAS (pid : nat) (old : nat) (new : nat)
-  | RegRead (pid : nat)
+  | RegCAS (old : nat) (new : nat)
+  | RegRead
   .
 
   Inductive Register_reply :=
-  | RegCASOk (pid : nat) (success : bool)
-  | RegReadOk (pid : nat) (value : nat)
+  | RegCASOk (success : bool)
+  | RegReadOk (value : nat)
   .
+
+  Definition li_register_valid_query_reply :=
+    fun q r => match q, r with
+    | RegCAS _ _, RegCASOk _ => True
+    | RegRead, RegReadOk _ => True
+    | _, _ => False
+    end.
 
   Definition li_register :=
     {|
       query := Register_query;
       reply := Register_reply;
+      valid_query_reply := li_register_valid_query_reply;
     |}.
 
   Inductive Internal := 
   | int_cas
   | int_read.
 
-  Inductive Invocation :=
+  (* Inductive Invocation :=
   | Inv_CAS (old : nat) (new : nat)
   | Inv_Read.
 
   Inductive Response :=
   | Res_CAS (success : bool)
-  | Res_Read (value : nat).
+  | Res_Read (value : nat). *)
 
   (* 
     A register state comprises of
@@ -61,8 +69,8 @@ Section Register.
     LibEnv.env T := list (nat*T)
   *)
   Record Register_state := mkRegState {
-    requests : LibEnv.env Invocation; 
-    responses : LibEnv.env Response;
+    requests : LibEnv.env Register_query; 
+    responses : LibEnv.env Register_reply;
     value : nat
   }.
 
@@ -75,57 +83,57 @@ Section Register.
   (* 
     Called by environment
   *)
-  Inductive register_initial_state : Register_state -> query li_register -> Register_state -> Prop :=
+  Inductive register_initial_state : Register_state -> Pid -> query li_register -> Register_state -> Prop :=
   | register_initial_state_cas : forall pid old new st st' inv res v,
     pid # inv -> pid # res ->
     st = mkRegState inv res v ->
-    st' = mkRegState ((pid, Inv_CAS old new)::inv) res v ->
-    register_initial_state st (RegCAS pid old new) st'
+    st' = mkRegState ((pid, RegCAS old new)::inv) res v ->
+    register_initial_state st pid (RegCAS old new) st'
   | register_initial_state_read : forall pid st st' inv res v,
     pid # inv -> pid # res ->
     st = mkRegState inv res v ->
-    st' = mkRegState ((pid, Inv_Read)::inv) res v ->
-    register_initial_state st (RegRead pid) st'
+    st' = mkRegState ((pid, RegRead)::inv) res v ->
+    register_initial_state st pid (RegRead) st'
   .
 
   (* 
     Return to environment
   *)
-  Inductive register_final_state : Register_state -> reply li_register -> Register_state -> Prop :=
+  Inductive register_final_state : Register_state -> Pid -> reply li_register -> Register_state -> Prop :=
   | register_final_state_cas : forall pid inv res res' res'' b v st st',
-    res = res' ++ [(pid, Res_CAS b)] ++ res'' ->
+    res = res' ++ [(pid, RegCASOk b)] ++ res'' ->
     st = mkRegState inv res v ->
     st' = mkRegState inv (res' ++ res'') v ->
-    register_final_state st (RegCASOk pid b) st'
+    register_final_state st pid (RegCASOk b) st'
   | register_final_state_read : forall pid inv res res' res'' v st st' ret,
-    res = res' ++ [(pid, Res_Read ret)] ++ res'' ->
+    res = res' ++ [(pid, RegReadOk ret)] ++ res'' ->
     st = mkRegState inv res v ->
     st' = mkRegState inv (res' ++ res'') v ->
-    register_final_state st (RegReadOk pid ret) st'
+    register_final_state st pid (RegReadOk ret) st'
   .
 
   (* 
     Internal execution
   *)
-  Inductive register_step : Register_state -> Internal -> Register_state -> Prop :=
+  Inductive register_step : Register_state -> Pid -> Internal -> Register_state -> Prop :=
   | register_step_cas : forall pid st st' inv inv' inv'' res v old new,
-    inv = inv' ++ [(pid, Inv_CAS old new)] ++ inv'' ->
+    inv = inv' ++ [(pid, RegCAS old new)] ++ inv'' ->
     st = mkRegState inv res v ->
-    st' = mkRegState (inv' ++ inv'') ((pid, Res_CAS (st.(value) =? old))::res) (if value st =? old then new else old) ->
-    register_step st int_cas st'
+    st' = mkRegState (inv' ++ inv'') ((pid, RegCASOk (st.(value) =? old))::res) (if value st =? old then new else old) ->
+    register_step st pid int_cas st'
   | register_step_read : forall pid st st' inv inv' inv'' res v,
-    inv = inv' ++ [(pid, Inv_Read)] ++ inv'' ->
+    inv = inv' ++ [(pid, RegRead)] ++ inv'' ->
     st = mkRegState inv res v ->
-    st' = mkRegState (inv' ++ inv'') ((pid, Res_Read v)::res) v ->
-    register_step st int_read st' 
+    st' = mkRegState (inv' ++ inv'') ((pid, RegReadOk v)::res) v ->
+    register_step st pid int_read st' 
   .
 
   (* 
     No external calls since Register does not rely on other objects
   *)
-  Inductive register_at_external : Register_state -> query li_null -> Register_state -> Prop :=.
+  Inductive register_at_external : Register_state -> Pid -> query li_null -> Register_state -> Prop :=.
 
-  Inductive register_after_external : Register_state -> reply li_null -> Register_state -> Prop :=.
+  Inductive register_after_external : Register_state -> Pid -> reply li_null -> Register_state -> Prop :=.
 
   Definition Register : lts li_null li_register  := mkLTS li_null li_register
     Register_state
